wip

Otbn/Examples/FeMul25519.v
@@ -17,8 +17,6 @@ Require Import coqutil.Word.LittleEndianList.
 Require Import coqutil.Z.PushPullMod.
 Require Import coqutil.Z.ZLib.
 Require Import Otbn.ISA.ISA.
-Require Import Otbn.Lib.Bignum.
-Require Import Otbn.Lib.BignumProperties.
 Require Import Otbn.Semantics.Clobbers.
 Require Import Otbn.Semantics.Semantics.
 Require Import Otbn.Semantics.Properties.
@@ -60,6 +58,31 @@ Section Defs.
     ("fe_mul"%string,
       map.empty,
       [[
+          (* Partial products for multiply-reduce:
+           *
+           * | a0b0    | a0b1    | a0b2    | a0b3 |
+           * |         | a1b0    | a1b1    | a1b2 |
+           * |         |         | a2b0    | a2b1 |
+           * |         |         |         | a3b0 |
+           * |         |         |         |      |
+           * | a1b3*38 | a2b3*38 | a3b3*38 |      |
+           * | a2b2*38 | a3b2*38 |         |      |
+           * | a3b1*38 |         |         |      |
+           *
+           * We can further optimize by computing the highest-weight partial products
+           * as t = (a0b2 + a1b1 + a2b0 + a3b3*38 + (a0b3 + a1b2 + a2b1 + a3b0) << 64)
+           * ahead of time and multiplying the upper half by 38 as well:
+           *
+           * | a0b0       | a0b1    | t0 | t1 |
+           * |            | a1b0    |    |    |
+           * |            |         |    |    |
+           * |            |         |    |    |
+           * |            |         |    |    |
+           * | a1b3*38    | a2b3*38 |    |    |
+           * | a2b2*38    | a3b2*38 |    |    |
+           * | a3b1*38    | t3*38   |    |    |
+           * | t2*38      |         |    |    |
+           *)
           (* Precompute b3*38 at an offset of 128 and store in w18 (this step also
              clears the lower part of w18, which is important later).
                w18.U <= b3*38 *)
@@ -67,7 +90,7 @@ Section Defs.
           (* Accumulate partial products from the top two limbs first, and store the
              result in ACC and w21.U such that:
                ACC <= t2 + t3 << 64
-               w21 <= t0 << 128 + t1 << 192 *)
+               w18 <= t0 << 128 + t1 << 192 *)
           bn.mulqacc.z          w22.0, w23.2, 0; (* a0b2 *)
           bn.mulqacc            w22.1, w23.1, 0; (* a1b1 *)
           bn.mulqacc            w22.2, w23.0, 0; (* a2b0 *)
@@ -79,7 +102,7 @@ Section Defs.
           bn.mulqacc.so  w18.U, w22.3, w18.3, 64, FG0; (* a3*((b3*38) >> 64) *)
           (* Reduce the high part modulo p. This guarantees a full reduction because
              the written-back value is at most (2^128 - 1) * 2^128 < 2 * p.
-               w18 <= (t0 + t1 << 64) mod p *)
+               w18 <= (t0 << 128 + t1 << 192) mod p *)
           bn.addm    w18, w18, w31;
           (* Accumulate partial products that need to be multiplied by 38 and are
              fully within the first 256 bits of the result. Result max. 194 bits.
@@ -109,3 +132,161 @@ Section Defs.
           ret ]]%otbn).
 
 End Defs.
+
+Section Math.
+  Local Infix "<<" := Z.shiftl (at level 40) : Z_scope.
+  Local Infix ">>" := Z.shiftr (at level 40) : Z_scope.
+
+  Definition p : Z := 2^255 - 19.
+
+  Definition to_limb64 (x : Z) : Z * Z * Z * Z :=
+    let x0 := x mod 2^64 in
+    let x1 := (x >> 64) mod 2^64 in
+    let x2 := (x >> 128) mod 2^64 in
+    let x3 := (x >> 192) mod 2^64 in
+    (x0, x1, x2, x3).
+
+  (* TODO: derive this part *)
+  Definition fe_mul_spec a b : Z :=
+    let '(a0, a1, a2, a3) := to_limb64 a in
+    let '(b0, b1, b2, b3) := to_limb64 b in
+    let hi := mulqacc_spec 0 b3 38 128 in
+    let acc := mulqacc_spec 0 a0 b2 0 in
+    let acc := mulqacc_spec acc a0 b2 0 in
+    let acc := mulqacc_spec acc a1 b1 0 in
+    let acc := mulqacc_spec acc a3 (hi >> 64) 0 in
+    let acc := mulqacc_spec acc a0 b3 64 in
+    let acc := mulqacc_spec acc a1 b2 64 in
+    let acc := mulqacc_spec acc a2 b1 64 in
+    let acc := mulqacc_spec acc a3 b0 64 in
+    let acc := mulqacc_spec acc a3 b0 64 in
+    let hi := so_writeback_spec true hi acc in
+    let acc := acc >> 128 in
+    let hi := addm_spec hi 0 p in
+    let acc := mulqacc_spec acc a1 b3 0 in
+    let acc := mulqacc_spec acc a2 b2 0 in
+    let acc := mulqacc_spec acc a3 b1 0 in
+    let acc := mulqacc_spec acc a2 b3 64 in
+    let acc := mulqacc_spec acc a3 b2 64 in
+    let lo := acc in
+    let acc := mulqacc_spec 0 lo 38 0 in
+    let acc := mulqacc_spec acc lo 38 64 in
+    let acc := mulqacc_spec acc lo 38 128 in
+    let acc := mulqacc_spec acc lo 38 192 in
+    let acc := mulqacc_spec acc a0 b0 0 in
+    let acc := mulqacc_spec acc a0 b1 64 in
+    let acc := mulqacc_spec acc a1 b0 64 in
+    let lo := acc in
+    let r := addm_spec lo hi p in
+    r.
+
+  (*
+    let b3_38 := b3 * 38 in
+    let t := a0 * b2 + a1 * b1 + a2 * b0 + a3 * b3_38 in
+    let t := t + ((a0 * b3 + a1 * b2 + a2 * b1 + a3 * b0) << 64) in
+    let '(t0, t1, t2, t3) := to_limb64 t in
+    let high := (t0 + t1 << 64) << 128 in
+    let high := if (p <? high) then (high - p) else high in
+    let low := a1 * b3 + a2 * b2 + a3 * b1 + t2 in
+    let low := low + ((a2 * b3 + a3 * b2 + t3) << 64) in
+    let low := low * 38 in
+    let low := low + (a0 * b0 + ((a0 * b1 + a1 * b0) << 64)) in
+    if (p <? low + high) then low + high - p else low + high.
+   *)
+
+  Lemma fe_mul_spec_correct a b :
+    0 <= a < 2^255 ->
+    0 <= b < 2^255 ->
+    fe_mul_spec a b = (a * b) mod p.
+  Admitted.
+  
+End Math.
+
+Section Proofs.
+  Context {word32 : word.word 32} {word32_ok : word.ok word32}.
+  Context {word256 : word.word 256} {word256_ok : word.ok word256}.
+  Context {regfile : map.map reg word32} {regfile_ok : map.ok regfile}.
+  Context {wregfile : map.map wreg word256} {wregfile_ok : map.ok wregfile}.
+  Context {flagfile : map.map flag bool} {flagfile_ok : map.ok flagfile}.
+  Context {mem : map.map word32 byte} {mem_ok : map.ok mem}.
+  Add Ring wring32: (@word.ring_theory 32 word32 word32_ok).
+  Add Ring wring256: (@word.ring_theory 256 word256 word256_ok).
+
+  (*
+  (* TODO: move *)
+  Lemma addm_full_reduce x y m :
+    word.unsigned x + word.unsigned y < 2 * m ->
+    word.unsigned (addm_spec x y (word.of_Z m)) = (word.unsigned x + word.unsigned y) mod m.
+  Admitted.
+   *)
+
+  Lemma fe_mul_correct regs wregs flags dmem cstack lstack a b :
+    (* @param[in]  w22: a, first operand, a < 2^255 *)
+    0 <= word.unsigned a < 2^255 ->
+    map.get wregs (wdreg w22) = Some a ->
+    (* @param[in]  w23: b, second operand, b < 2^255 *)
+    0 <= word.unsigned b < 2^255 ->
+    map.get wregs (wdreg w23) = Some b ->
+    (* @param[in]  w30: constant, 38 *)
+    map.get wregs (wdreg w30) = Some (word.of_Z 38) ->
+    (* @param[in]  w31: all-zero *)
+    map.get wregs (wdreg w31) = Some (word.of_Z 0) ->
+    (* @param[in]  MOD: p, modulus = 2^255 - 19 *)
+    map.get wregs (wsreg WSR_MOD) = Some (word.of_Z p) ->
+    returns
+      (fetch:=fetch_ctx [fe_mul])
+      "fe_mul"%string regs wregs flags dmem cstack lstack
+      (fun regs' wregs' flags' dmem' =>
+         dmem = dmem'
+         /\ (exists v,
+                map.get wregs' (wdreg w22) = Some v
+                /\ word.unsigned v = (word.unsigned a * word.unsigned b) mod p)
+         (* clobbered registers: w18, w20 to w22 *)
+         /\ clobbers [wdreg w18; wdreg w20; wdreg w21; wdreg w22; wsreg WSR_ACC] wregs wregs'
+         /\ clobbers [] regs regs'
+         (* clobbered flag groups: FG0 *)
+         /\ clobbers [flagM FG0; flagL FG0; flagZ FG0; flagC FG0] flags flags').
+  Proof.
+    cbv [returns fe_mul]; intros; subst.
+    repeat straightline_step.
+    eapply eventually_ret; [ reflexivity | eassumption | ].
+    ssplit; try reflexivity; [ | solve_clobbers .. ].
+    eexists; ssplit; [ eassumption | ].
+
+    (* here we have to prove the math! *)
+    etransitivity; [ | apply fe_mul_spec_correct; lia ].
+
+    (* all the flags should be irrelevant, clear them to clean up the context *)
+    lazymatch goal with
+    | x := _ : bool |- _ => clear dependent x
+    end.
+
+    (* helpful assertion *)
+    assert (p < 2^256) by (exact eq_refl).
+
+    (* unfold fe_mul_spec and introduce all its lets *)
+    cbv beta delta [fe_mul_spec].
+    repeat lazymatch goal with
+           | |- ?lhs = (match ?e with pair x y => ?f end) =>
+               rewrite (surjective_pairing e); cbn iota;
+               change (let x := fst e in let y := snd e in lhs = f); do 2 intro
+           | |- ?lhs = (let x := ?e in ?f) =>
+               change (let x := e in lhs = f); intro
+           end.
+
+    subst v37.
+    lazymatch goal with
+    | |- word.unsigned (addm_spec ?x ?y (word.of_Z ?m)) = (?a + ?b) mod ?m =>
+        replace a with (word.unsigned x); [ replace b with (word.unsigned y) | ];
+        [ apply addm_full_reduce | .. ]
+    end.
+    {
+      apply addm_full_reduce.
+    rewrite addm_full_reduce.
+    rewrite word.unsigned_of_Z_nowrap by lia.
+    Search addm_spec.
+    
+  Qed.
+
+
+End Proofs.
